@prefix : <http://www.semanticweb.org/ivans/ontologies/2025/cps-code-generation/> .
@prefix owl: <http://www.w3.org/2002/07/owl#> .
@prefix rdf: <http://www.w3.org/1999/02/22-rdf-syntax-ns#> .
@prefix xml: <http://www.w3.org/XML/1998/namespace> .
@prefix xsd: <http://www.w3.org/2001/XMLSchema#> .
@prefix rdfs: <http://www.w3.org/2000/01/rdf-schema#> .
@base <http://www.semanticweb.org/ivans/ontologies/2025/cps-code-generation/> .

<http://www.semanticweb.org/ivans/ontologies/2025/cps-code-generation> rdf:type owl:Ontology ;
                                                                        owl:imports <http://www.w3.org/ns/ssn/systems/> .

#################################################################
#    Datatypes
#################################################################

###  http://www.semanticweb.org/ivans/ontologies/2025/cps-code-generation/testType
:testType rdf:type rdfs:Datatype .


#################################################################
#    Object Properties
#################################################################

###  http://www.semanticweb.org/ivans/ontologies/2025/cps-code-generation#affects
:affects rdf:type owl:ObjectProperty ;
         rdfs:domain :ActuatorState ;
         rdfs:range <http://www.w3.org/ns/sosa/ObservableProperty> ;
         rdfs:comment "Represents that a given actuator state has an effect on a given property."@en ;
         rdfs:label "affects"@en .


###  http://www.w3.org/ns/ssn/forProperty
<http://www.w3.org/ns/ssn/forProperty> rdfs:range <http://www.w3.org/ns/ssn/Property> .


#################################################################
#    Data properties
#################################################################

###  http://www.semanticweb.org/ivans/ontologies/2025/cps-code-generation#decreasesBy
:decreasesBy rdf:type owl:DatatypeProperty ;
             rdfs:domain :ActuatorState ;
             rdfs:range xsd:double ;
             rdfs:comment "Denotes an actuator state's decrease of a given property's value by a certain amount."@en ;
             rdfs:label "decreasesBy"@en .


###  http://www.semanticweb.org/ivans/ontologies/2025/cps-code-generation#hasComputationFMU
:hasComputationFMU rdf:type owl:DatatypeProperty ;
                   rdfs:subPropertyOf :hasModel ;
                   rdfs:range xsd:anyURI ;
                   rdfs:comment "Refers to an FMU to be used for computations or modeling."@en ;
                   rdfs:label "hasComputationFMU"@en .


###  http://www.semanticweb.org/ivans/ontologies/2025/cps-code-generation#hasDataSanitizationFMU
:hasDataSanitizationFMU rdf:type owl:DatatypeProperty ;
                        rdfs:subPropertyOf :hasModel ;
                        rdfs:range xsd:anyURI ;
                        rdfs:comment "Refers to an FMU to be used for data sanitization."@en ;
                        rdfs:label "hasDataSanitizationFMU"@en .


###  http://www.semanticweb.org/ivans/ontologies/2025/cps-code-generation#hasModel
:hasModel rdf:type owl:DatatypeProperty ;
          rdfs:domain <http://www.w3.org/ns/sosa/Procedure> ;
          rdfs:range xsd:anyURI ;
          rdfs:comment "Refers to a model, such as a functional mock-up unit (FMU), used by a given Procedure."@en ;
          rdfs:label "hasModel"@en .


###  http://www.semanticweb.org/ivans/ontologies/2025/cps-code-generation#increasesBy
:increasesBy rdf:type owl:DatatypeProperty ;
             rdfs:domain :ActuatorState ;
             rdfs:range xsd:double ;
             rdfs:comment "Denotes an actuator state's increase of a given property's value by a certain amount."@en ;
             rdfs:label "increasesBy"@en .


###  http://www.semanticweb.org/ivans/ontologies/2025/cps-code-generation#setsTo
:setsTo rdf:type owl:DatatypeProperty ;
        rdfs:domain :ActuatorState ;
        rdfs:range rdfs:Literal ;
        rdfs:comment "A range of possible property values set by a given actuator state."@en ;
        rdfs:label "setsTo"@en .


#################################################################
#    Classes
#################################################################

###  http://www.semanticweb.org/ivans/ontologies/2025/cps-code-generation#NonOptimalCondition
:NonOptimalCondition rdf:type owl:Class ;
                     rdfs:subClassOf <http://www.w3.org/ns/ssn/systems/Condition> ,
                                     [ rdf:type owl:Restriction ;
                                       owl:onProperty <http://www.w3.org/ns/ssn/forProperty> ;
                                       owl:qualifiedCardinality "1"^^xsd:nonNegativeInteger ;
                                       owl:onClass <http://www.w3.org/ns/sosa/ObservableProperty>
                                     ] ;
                     owl:disjointWith :OptimalCondition ;
                     rdfs:comment "A non-optimal property condition, such as an undesired value range definition. For example, a non-optimal temperature condition of a room could be defined as values greater than 22 degrees Celsius."@en ;
                     rdfs:label "NonOptimalCondition"@en .


###  http://www.semanticweb.org/ivans/ontologies/2025/cps-code-generation#OptimalCondition
:OptimalCondition rdf:type owl:Class ;
                  rdfs:subClassOf <http://www.w3.org/ns/ssn/systems/Condition> ,
                                  [ rdf:type owl:Restriction ;
                                    owl:onProperty <http://www.w3.org/ns/ssn/forProperty> ;
                                    owl:qualifiedCardinality "1"^^xsd:nonNegativeInteger ;
                                    owl:onClass <http://www.w3.org/ns/sosa/ObservableProperty>
                                  ] ;
                  rdfs:comment "An optimal property condition, such as a desired value range definition. For example, an optimal temperature condition of a room could be defined as values greater than 18 and less than 22 degrees Celsius." ;
                  rdfs:label "OptimalCondition"@en .


###  http://www.semanticweb.org/ivans/ontologies/2025/cps-code-generation/ActuatorState
:ActuatorState rdf:type owl:Class ;
               rdfs:subClassOf [ rdf:type owl:Restriction ;
                                 owl:onProperty :affects ;
                                 owl:qualifiedCardinality "1"^^xsd:nonNegativeInteger ;
                                 owl:onClass <http://www.w3.org/ns/sosa/ObservableProperty>
                               ] ;
               rdfs:comment "The state of a given actuator, such as \"On\" or \"Off\" for a simple cooling fan or a specific temperature setting of an AC unit."@en ;
               rdfs:label "ActuatorState"@en .


###  Generated by the OWL API (version 4.5.29.2024-05-13T12:11:03Z) https://github.com/owlcs/owlapi
