@prefix : <http://www.semanticweb.org/ivans/ontologies/2025/cps-code-generation/> .
@prefix owl: <http://www.w3.org/2002/07/owl#> .
@prefix rdf: <http://www.w3.org/1999/02/22-rdf-syntax-ns#> .
@prefix xml: <http://www.w3.org/XML/1998/namespace> .
@prefix xsd: <http://www.w3.org/2001/XMLSchema#> .
@prefix rdfs: <http://www.w3.org/2000/01/rdf-schema#> .
@base <http://www.semanticweb.org/ivans/ontologies/2025/cps-code-generation/> .

<http://www.semanticweb.org/ivans/ontologies/2025/cps-code-generation> rdf:type owl:Ontology ;
                                                                        owl:imports <http://www.w3.org/ns/ssn/systems/> .

#################################################################
#    Datatypes
#################################################################

###  http://www.w3.org/2001/XMLSchema#duration
xsd:duration rdf:type rdfs:Datatype .


#################################################################
#    Object Properties
#################################################################

###  http://www.semanticweb.org/ivans/ontologies/2025/cps-code-generation/affectsPropertyWith
:affectsPropertyWith rdf:type owl:ObjectProperty ;
                     rdfs:range :Effect ;
                     rdfs:comment "Represents that a given actuator state has an effect on a given property."@en ;
                     rdfs:label "affectsPropertyWith"@en .


###  http://www.semanticweb.org/ivans/ontologies/2025/cps-code-generation/hasActuatorState
:hasActuatorState rdf:type owl:ObjectProperty ;
                  owl:inverseOf :isStateOf ;
                  rdfs:domain <http://www.w3.org/ns/sosa/Actuator> ;
                  rdfs:range :ActuatorState ;
                  rdfs:label "Represents the relation between an actuator and its state."@en ,
                             "hasActuatorState"@en .


###  http://www.semanticweb.org/ivans/ontologies/2025/cps-code-generation/isOutputOf
:isOutputOf rdf:type owl:ObjectProperty ;
            owl:inverseOf <http://www.w3.org/ns/ssn/hasOutput> ;
            rdfs:comment "Relation between an Output and its Procedure."@en ;
            rdfs:label "isOutputOf"@en .


###  http://www.semanticweb.org/ivans/ontologies/2025/cps-code-generation/isStateOf
:isStateOf rdf:type owl:ObjectProperty ;
           rdfs:comment "Relation between an ActuatorState and its Actuator."@en ;
           rdfs:label "isStateOf"@en .


###  http://www.semanticweb.org/ivans/ontologies/2025/cps-code-generation/isSubsystemOf
:isSubsystemOf rdf:type owl:ObjectProperty ;
               owl:inverseOf <http://www.w3.org/ns/ssn/hasSubSystem> ;
               rdfs:comment "Relation between a subsystem and its System."@en ;
               rdfs:label "isSubsystemOf"@en .


###  http://www.semanticweb.org/ivans/ontologies/2025/cps-code-generation/withActuator
:withActuator rdf:type owl:ObjectProperty ;
              rdfs:domain :MitigationStrategy ;
              rdfs:range <http://www.w3.org/ns/sosa/Actuator> ;
              rdfs:comment "The relation between a MitigationStrategy and an Actuator it uses."@en ;
              rdfs:label "withActuator"@en .


###  http://www.semanticweb.org/ivans/ontologies/2025/cps-code-generation/withActuatorState
:withActuatorState rdf:type owl:ObjectProperty ;
                   rdfs:domain :MitigationStrategy ;
                   rdfs:range :ActuatorState ;
                   rdfs:comment "The relation between a MitigationStrategy and an ActuatorState it uses."@en ;
                   rdfs:label "withActuatorState"@en .


###  http://www.w3.org/ns/ssn/forProperty
<http://www.w3.org/ns/ssn/forProperty> rdfs:range <http://www.w3.org/ns/ssn/Property> .


#################################################################
#    Data properties
#################################################################

###  http://www.semanticweb.org/ivans/ontologies/2025/cps-code-generation/hasComputationFMU
:hasComputationFMU rdf:type owl:DatatypeProperty ;
                   rdfs:subPropertyOf :hasModel ;
                   rdfs:range xsd:anyURI ;
                   rdfs:comment "Refers to an FMU to be used for computations or modeling."@en ;
                   rdfs:label "hasComputationFMU"@en .


###  http://www.semanticweb.org/ivans/ontologies/2025/cps-code-generation/hasDataSanitizationFMU
:hasDataSanitizationFMU rdf:type owl:DatatypeProperty ;
                        rdfs:subPropertyOf :hasModel ;
                        rdfs:range xsd:anyURI ;
                        rdfs:comment "Refers to an FMU to be used for data sanitization."@en ;
                        rdfs:label "hasDataSanitizationFMU"@en .


###  http://www.semanticweb.org/ivans/ontologies/2025/cps-code-generation/hasModel
:hasModel rdf:type owl:DatatypeProperty ;
          rdfs:domain <http://www.w3.org/ns/sosa/Procedure> ;
          rdfs:range xsd:anyURI ;
          rdfs:comment "Refers to a model, such as a functional mock-up unit (FMU), used by a given Procedure."@en ;
          rdfs:label "hasModel"@en .


###  http://www.semanticweb.org/ivans/ontologies/2025/cps-code-generation/hasValueConstraint
:hasValueConstraint rdf:type owl:DatatypeProperty ;
                    rdfs:range xsd:double ;
                    rdfs:comment "Represents the relation between a thing and its defined range of values."@en ;
                    rdfs:label "hasValueConstraint"@en .


###  http://www.semanticweb.org/ivans/ontologies/2025/cps-code-generation/hasValueType
:hasValueType rdf:type owl:DatatypeProperty ;
              rdfs:range rdfs:Literal ;
              rdfs:comment "Describes a relation to a specific value type used by a property or an input/output parameter."@en ;
              rdfs:label "hasValueType"@en .


###  http://www.semanticweb.org/ivans/ontologies/2025/cps-code-generation/withTimeLimit
:withTimeLimit rdf:type owl:DatatypeProperty ;
               rdfs:domain :MitigationStrategy ;
               rdfs:range xsd:duration ;
               rdfs:comment "Represents a time limit on the duration of the MitigationStrategy."@en ;
               rdfs:label "withTimeLimit"@en .


#################################################################
#    Classes
#################################################################

###  http://www.semanticweb.org/ivans/ontologies/2025/cps-code-generation#ConfigurableProperty
:ConfigurableProperty rdf:type owl:Class ;
                      rdfs:subClassOf <http://www.w3.org/ns/ssn/Property> ,
                                      [ rdf:type owl:Restriction ;
                                        owl:onProperty :hasValueType ;
                                        owl:cardinality "1"^^xsd:nonNegativeInteger
                                      ] ;
                      rdfs:comment "A property not directly observable or actuatable but rather used for configuring a System or Procedure."@en ;
                      rdfs:label "ConfigurableProperty"@en .


###  http://www.semanticweb.org/ivans/ontologies/2025/cps-code-generation/ActuatorState
:ActuatorState rdf:type owl:Class ;
               rdfs:subClassOf [ rdf:type owl:Restriction ;
                                 owl:onProperty :affectsPropertyWith ;
                                 owl:qualifiedCardinality "1"^^xsd:nonNegativeInteger ;
                                 owl:onClass :Effect
                               ] ,
                               [ rdf:type owl:Restriction ;
                                 owl:onProperty :isStateOf ;
                                 owl:qualifiedCardinality "1"^^xsd:nonNegativeInteger ;
                                 owl:onClass <http://www.w3.org/ns/sosa/Actuator>
                               ] ;
               rdfs:comment "The state of a given actuator, such as \"On\" or \"Off\" for a simple cooling fan or a specific temperature setting of an AC unit."@en ;
               rdfs:label "ActuatorState"@en .


###  http://www.semanticweb.org/ivans/ontologies/2025/cps-code-generation/Decrease
:Decrease rdf:type owl:Class ;
          rdfs:subClassOf :Effect ;
          rdfs:comment "Represents a decrease in the value of a property."@en ;
          rdfs:label "Decrease"@en .


###  http://www.semanticweb.org/ivans/ontologies/2025/cps-code-generation/Effect
:Effect rdf:type owl:Class ;
        rdfs:subClassOf [ rdf:type owl:Restriction ;
                          owl:onProperty <http://www.w3.org/ns/ssn/forProperty> ;
                          owl:minQualifiedCardinality "1"^^xsd:nonNegativeInteger ;
                          owl:onClass <http://www.w3.org/ns/sosa/ObservableProperty>
                        ] ;
        rdfs:comment "The type of effect an actuator state has on the value of a property."@en ;
        rdfs:label "Effect"@en .


###  http://www.semanticweb.org/ivans/ontologies/2025/cps-code-generation/Increase
:Increase rdf:type owl:Class ;
          rdfs:subClassOf :Effect ;
          rdfs:comment "Represents an increase in the value of a property."@en ;
          rdfs:label "Increase"@en .


###  http://www.semanticweb.org/ivans/ontologies/2025/cps-code-generation/MitigationStrategy
:MitigationStrategy rdf:type owl:Class ;
                    rdfs:subClassOf <http://www.w3.org/ns/sosa/Procedure> ,
                                    [ rdf:type owl:Restriction ;
                                      owl:onProperty :withActuator ;
                                      owl:minQualifiedCardinality "1"^^xsd:nonNegativeInteger ;
                                      owl:onClass <http://www.w3.org/ns/sosa/Actuator>
                                    ] ,
                                    [ rdf:type owl:Restriction ;
                                      owl:onProperty :withActuatorState ;
                                      owl:minQualifiedCardinality "1"^^xsd:nonNegativeInteger ;
                                      owl:onClass :ActuatorState
                                    ] ,
                                    [ rdf:type owl:Restriction ;
                                      owl:onProperty :withTimeLimit ;
                                      owl:minQualifiedCardinality "1"^^xsd:nonNegativeInteger ;
                                      owl:onDataRange xsd:duration
                                    ] ;
                    rdfs:comment "Represents a strategy for regaining optimal conditions with some combination of appropriate actuators, their states, and given actuation durations."@en ;
                    rdfs:label "MitigationStrategy"@en .


###  http://www.semanticweb.org/ivans/ontologies/2025/cps-code-generation/NonOptimalCondition
:NonOptimalCondition rdf:type owl:Class ;
                     rdfs:subClassOf <http://www.w3.org/ns/ssn/systems/Condition> ,
                                     [ rdf:type owl:Restriction ;
                                       owl:onProperty <http://www.w3.org/ns/ssn/forProperty> ;
                                       owl:qualifiedCardinality "1"^^xsd:nonNegativeInteger ;
                                       owl:onClass <http://www.w3.org/ns/sosa/ObservableProperty>
                                     ] ;
                     owl:disjointWith :OptimalCondition ;
                     rdfs:comment "A non-optimal property condition, such as an undesired value range definition. For example, a non-optimal temperature condition of a room could be defined as values greater than 22 degrees Celsius."@en ;
                     rdfs:label "NonOptimalCondition"@en .


###  http://www.semanticweb.org/ivans/ontologies/2025/cps-code-generation/OptimalCondition
:OptimalCondition rdf:type owl:Class ;
                  rdfs:subClassOf <http://www.w3.org/ns/ssn/systems/Condition> ,
                                  [ rdf:type owl:Restriction ;
                                    owl:onProperty <http://www.w3.org/ns/ssn/forProperty> ;
                                    owl:qualifiedCardinality "1"^^xsd:nonNegativeInteger ;
                                    owl:onClass <http://www.w3.org/ns/sosa/ObservableProperty>
                                  ] ;
                  rdfs:comment "An optimal property condition, such as a desired value range definition. For example, an optimal temperature condition of a room could be defined as values greater than 18 and less than 22 degrees Celsius." ;
                  rdfs:label "OptimalCondition"@en .


###  http://www.w3.org/ns/sosa/Actuator
<http://www.w3.org/ns/sosa/Actuator> rdfs:subClassOf [ rdf:type owl:Restriction ;
                                                       owl:onProperty :hasActuatorState ;
                                                       owl:minQualifiedCardinality "1"^^xsd:nonNegativeInteger ;
                                                       owl:onClass :ActuatorState
                                                     ] .


###  http://www.w3.org/ns/sosa/ObservableProperty
<http://www.w3.org/ns/sosa/ObservableProperty> rdfs:subClassOf [ rdf:type owl:Restriction ;
                                                                 owl:onProperty :hasValueType ;
                                                                 owl:cardinality "1"^^xsd:nonNegativeInteger
                                                               ] .


###  Generated by the OWL API (version 4.5.29.2024-05-13T12:11:03Z) https://github.com/owlcs/owlapi
