@prefix : <http://www.semanticweb.org/ivans/ontologies/2025/dt-code-generation/> .
@prefix owl: <http://www.w3.org/2002/07/owl#> .
@prefix rdf: <http://www.w3.org/1999/02/22-rdf-syntax-ns#> .
@prefix xml: <http://www.w3.org/XML/1998/namespace> .
@prefix xsd: <http://www.w3.org/2001/XMLSchema#> .
@prefix rdfs: <http://www.w3.org/2000/01/rdf-schema#> .
@base <http://www.semanticweb.org/ivans/ontologies/2025/dt-code-generation/> .

<http://www.semanticweb.org/ivans/ontologies/2025/dt-code-generation> rdf:type owl:Ontology ;
                                                                       owl:imports <http://www.w3.org/ns/ssn/systems/> .

#################################################################
#    Datatypes
#################################################################

###  http://www.w3.org/2001/XMLSchema#duration
xsd:duration rdf:type rdfs:Datatype .


#################################################################
#    Object Properties
#################################################################

###  http://www.semanticweb.org/ivans/ontologies/2025/dt-code-generation/affectsPropertyWith
:affectsPropertyWith rdf:type owl:ObjectProperty ;
                     rdfs:range :Effect ;
                     rdfs:comment "Represents that a Thing has an effect on a Property."@en ;
                     rdfs:label "affectsPropertyWith"@en .


###  http://www.semanticweb.org/ivans/ontologies/2025/dt-code-generation/alteredBy
:alteredBy rdf:type owl:ObjectProperty ;
           rdfs:domain :PropertyChangeByReconfiguration ;
           rdfs:range :Effect ;
           rdfs:comment "Represents a relation between a ConfigurableProperty and an Effect on it that causes a related property to change."@en ;
           rdfs:label "alteredBy"@en .


###  http://www.semanticweb.org/ivans/ontologies/2025/dt-code-generation/enactedBy
:enactedBy rdf:type owl:ObjectProperty ;
           owl:inverseOf :enacts ;
           rdfs:comment "Represents a relation between a PropertyChange and a thing, such as a System or Actuator."@en ;
           rdfs:label "enactedBy"@en .


###  http://www.semanticweb.org/ivans/ontologies/2025/dt-code-generation/enacts
:enacts rdf:type owl:ObjectProperty ;
        rdfs:range :PropertyChange ;
        rdfs:comment "Represents a relation between a thing, such as a System or Actuator, and a PropertyChange."@en ;
        rdfs:label "enacts"@en .


###  http://www.semanticweb.org/ivans/ontologies/2025/dt-code-generation/hasActuator
:hasActuator rdf:type owl:ObjectProperty ;
             rdfs:domain :ActuationAction ;
             rdfs:range <http://www.w3.org/ns/sosa/Actuator> ;
             rdfs:comment "The relation between an ActuationExecution and an Actuator it uses."@en ;
             rdfs:label "hasActuator"@en .


###  http://www.semanticweb.org/ivans/ontologies/2025/dt-code-generation/hasActuatorState
:hasActuatorState rdf:type owl:ObjectProperty ;
                  owl:inverseOf :isActuatorStateOf ;
                  rdfs:range :ActuatorState ;
                  rdfs:comment "Represents a relation between an entity and an ActuatorState."@en ;
                  rdfs:label "hasActuatorState"@en .


###  http://www.semanticweb.org/ivans/ontologies/2025/dt-code-generation/isActuatorStateOf
:isActuatorStateOf rdf:type owl:ObjectProperty ;
                   rdfs:domain :ActuatorState ;
                   rdfs:comment "Represents the relation between an ActuatorState and an entity."@en ;
                   rdfs:label "isActuatorStateOf"@en .


###  http://www.semanticweb.org/ivans/ontologies/2025/dt-code-generation/isInputOf
:isInputOf rdf:type owl:ObjectProperty ;
           owl:inverseOf <http://www.w3.org/ns/ssn/hasInput> ;
           rdfs:comment "Relation between an Input and its Procedure."@en ;
           rdfs:label "isInputOf"@en .


###  http://www.semanticweb.org/ivans/ontologies/2025/dt-code-generation/isOutputOf
:isOutputOf rdf:type owl:ObjectProperty ;
            owl:inverseOf <http://www.w3.org/ns/ssn/hasOutput> ;
            rdfs:comment "Relation between an Output and its Procedure."@en ;
            rdfs:label "isOutputOf"@en .


###  http://www.semanticweb.org/ivans/ontologies/2025/dt-code-generation/optimizedBy
:optimizedBy rdf:type owl:ObjectProperty ;
             owl:inverseOf :optimizesFor ;
             rdfs:comment "A relation between a Property and a Platform optimizing for it."@en ;
             rdfs:label "optimizedBy"@en .


###  http://www.semanticweb.org/ivans/ontologies/2025/dt-code-generation/optimizesFor
:optimizesFor rdf:type owl:ObjectProperty ;
              rdfs:domain <http://www.w3.org/ns/sosa/Platform> ;
              rdfs:range :PropertyChange ;
              rdfs:comment "Represents a relation between a platform and a PropertyChange that indicates that platform's optimization of those properties."@en ;
              rdfs:label "optimizesFor"@en .


###  http://www.semanticweb.org/ivans/ontologies/2025/dt-code-generation/propertyFor
:propertyFor rdf:type owl:ObjectProperty ;
             owl:inverseOf <http://www.w3.org/ns/ssn/forProperty> ;
             rdfs:comment "A relation between some property and an entity."@en ;
             rdfs:label "property for"@en .


#################################################################
#    Data properties
#################################################################

###  http://www.semanticweb.org/ivans/ontologies/2025/dt-code-generation/altersBy
:altersBy rdf:type owl:DatatypeProperty ;
          rdfs:domain :ReconfigurationAction ;
          rdfs:range rdfs:Literal ;
          rdfs:comment "Represents the relation between a ReconfiguationAction and the literal (value) it alters a ConfigurableParameter with."@en ;
          rdfs:label "altersBy"@en .


###  http://www.semanticweb.org/ivans/ontologies/2025/dt-code-generation/hasIdentifier
:hasIdentifier rdf:type owl:DatatypeProperty ;
               rdfs:range xsd:string ;
               rdfs:comment "Represents a relation from a thing to its identifier."@en ;
               rdfs:label "hasIdentifier"@en .


###  http://www.semanticweb.org/ivans/ontologies/2025/dt-code-generation/hasLowerLimitValue
:hasLowerLimitValue rdf:type owl:DatatypeProperty ;
                    rdfs:subPropertyOf owl:topDataProperty ;
                    rdfs:range rdfs:Literal ;
                    rdfs:comment "Describes a relation to a specific value's lower limit (of a specific type) contained by a property or an Input/Output parameter."@en ;
                    rdfs:label "hasLowerLimitValue"@en .


###  http://www.semanticweb.org/ivans/ontologies/2025/dt-code-generation/hasModel
:hasModel rdf:type owl:DatatypeProperty ;
          rdfs:domain <http://www.w3.org/ns/sosa/Procedure> ;
          rdfs:range xsd:anyURI ;
          rdfs:comment "Refers to a model, such as a functional mock-up unit (FMU), used by a given Procedure."@en ;
          rdfs:label "hasModel"@en .


###  http://www.semanticweb.org/ivans/ontologies/2025/dt-code-generation/hasTimeLimit
:hasTimeLimit rdf:type owl:DatatypeProperty ;
              rdfs:range xsd:duration ;
              rdfs:comment "Represents a time limit on the duration of the Strategy."@en ;
              rdfs:label "hasTimeLimit"@en .


###  http://www.semanticweb.org/ivans/ontologies/2025/dt-code-generation/hasUpperLimitValue
:hasUpperLimitValue rdf:type owl:DatatypeProperty ;
                    rdfs:subPropertyOf owl:topDataProperty ;
                    rdfs:range rdfs:Literal ;
                    rdfs:comment "Describes a relation to a specific value's upper limit (of a specific type) contained by a property or an Input/Output parameter."@en ;
                    rdfs:label "hasUpperLimitValue"@en .


###  http://www.semanticweb.org/ivans/ontologies/2025/dt-code-generation/hasValue
:hasValue rdf:type owl:DatatypeProperty ;
          rdfs:range rdfs:Literal ;
          rdfs:comment "Describes a relation to a specific value (of a specific type) contained by a property or an Input/Output parameter."@en ;
          rdfs:label "hasValue"@en .


###  http://www.semanticweb.org/ivans/ontologies/2025/dt-code-generation/hasValueConstraint
:hasValueConstraint rdf:type owl:DatatypeProperty ;
                    rdfs:range rdfs:Literal ;
                    rdfs:comment "Represents the relation between a thing and its defined range of values."@en ;
                    rdfs:label "hasValueConstraint"@en .


###  http://www.semanticweb.org/ivans/ontologies/2025/dt-code-generation/reachedInMaximumSeconds
:reachedInMaximumSeconds rdf:type owl:DatatypeProperty ;
                         rdfs:domain :OptimalCondition ;
                         rdfs:range xsd:int ;
                         rdfs:comment "Represents the maximum amount of time in seconds to reach an OptimalCondition."@en ;
                         rdfs:label "reachedInMaximumSeconds"@en .


#################################################################
#    Classes
#################################################################

###  http://www.semanticweb.org/ivans/ontologies/2025/dt-code-generation/Action
:Action rdf:type owl:Class ;
        rdfs:comment "Represents a single system Action."@en ;
        rdfs:label "Action"@en .


###  http://www.semanticweb.org/ivans/ontologies/2025/dt-code-generation/ActuationAction
:ActuationAction rdf:type owl:Class ;
                 rdfs:subClassOf :Action ,
                                 [ rdf:type owl:Restriction ;
                                   owl:onProperty :hasActuatorState ;
                                   owl:qualifiedCardinality "1"^^xsd:nonNegativeInteger ;
                                   owl:onClass :ActuatorState
                                 ] ;
                 owl:disjointWith :ReconfigurationAction ;
                 rdfs:comment "Represents a single system Action with an actuation, either for optimization or regaining optimal conditions."@en ;
                 rdfs:label "ActuationAction"@en .


###  http://www.semanticweb.org/ivans/ontologies/2025/dt-code-generation/ActuatorState
:ActuatorState rdf:type owl:Class ;
               rdfs:subClassOf [ rdf:type owl:Restriction ;
                                 owl:onProperty :enacts ;
                                 owl:minQualifiedCardinality "1"^^xsd:nonNegativeInteger ;
                                 owl:onClass :PropertyChangeByActuation
                               ] ,
                               [ rdf:type owl:Restriction ;
                                 owl:onProperty :isActuatorStateOf ;
                                 owl:qualifiedCardinality "1"^^xsd:nonNegativeInteger ;
                                 owl:onClass <http://www.w3.org/ns/sosa/Actuator>
                               ] ;
               rdfs:comment "Represents a given state of an Actuator with a possible range of values."@en ;
               rdfs:label "ActuatorState"@en .


###  http://www.semanticweb.org/ivans/ontologies/2025/dt-code-generation/ConfigurableParameter
:ConfigurableParameter rdf:type owl:Class ;
                       rdfs:subClassOf <http://www.w3.org/ns/ssn/Input> ,
                                       [ rdf:type owl:Restriction ;
                                         owl:onProperty :enacts ;
                                         owl:minQualifiedCardinality "1"^^xsd:nonNegativeInteger ;
                                         owl:onClass :PropertyChangeByReconfiguration
                                       ] ,
                                       [ rdf:type owl:Restriction ;
                                         owl:onProperty :hasLowerLimitValue ;
                                         owl:cardinality "1"^^xsd:nonNegativeInteger
                                       ] ,
                                       [ rdf:type owl:Restriction ;
                                         owl:onProperty :hasUpperLimitValue ;
                                         owl:cardinality "1"^^xsd:nonNegativeInteger
                                       ] ;
                       rdfs:comment "A parameter not directly observable or actuatable but rather used for configuring an an Input to a System or Procedure."@en ;
                       rdfs:label "ConfigurableParameter"@en .


###  http://www.semanticweb.org/ivans/ontologies/2025/dt-code-generation/Effect
:Effect rdf:type owl:Class ;
        rdfs:comment "The type of effect on the value of a property."@en ;
        rdfs:label "Effect"@en .


###  http://www.semanticweb.org/ivans/ontologies/2025/dt-code-generation/OptimalCondition
:OptimalCondition rdf:type owl:Class ;
                  rdfs:subClassOf <http://www.w3.org/ns/ssn/systems/Condition> ,
                                  [ rdf:type owl:Restriction ;
                                    owl:onProperty <http://www.w3.org/ns/ssn/forProperty> ;
                                    owl:qualifiedCardinality "1"^^xsd:nonNegativeInteger ;
                                    owl:onClass <http://www.w3.org/ns/ssn/Property>
                                  ] ,
                                  [ rdf:type owl:Restriction ;
                                    owl:onProperty :hasValueConstraint ;
                                    owl:cardinality "1"^^xsd:nonNegativeInteger
                                  ] ,
                                  [ rdf:type owl:Restriction ;
                                    owl:onProperty :reachedInMaximumSeconds ;
                                    owl:maxQualifiedCardinality "1"^^xsd:nonNegativeInteger ;
                                    owl:onDataRange xsd:int
                                  ] ;
                  rdfs:comment "An optimal property condition, such as a desired value range definition. For example, an optimal temperature condition of a room could be defined as values greater than 18 and lower than 22 degrees Celsius."@en ;
                  rdfs:label "OptimalCondition"@en .


###  http://www.semanticweb.org/ivans/ontologies/2025/dt-code-generation/PropertyChange
:PropertyChange rdf:type owl:Class ;
                rdfs:subClassOf [ rdf:type owl:Restriction ;
                                  owl:onProperty :affectsPropertyWith ;
                                  owl:qualifiedCardinality "1"^^xsd:nonNegativeInteger ;
                                  owl:onClass :Effect
                                ] ,
                                [ rdf:type owl:Restriction ;
                                  owl:onProperty <http://www.w3.org/ns/ssn/forProperty> ;
                                  owl:qualifiedCardinality "1"^^xsd:nonNegativeInteger ;
                                  owl:onClass <http://www.w3.org/ns/ssn/Property>
                                ] ;
                rdfs:comment "Represents a specific property change in a given system, either via a changed configuration property or an actuation on an observable one."@en ;
                rdfs:label "PropertyChange"@en .


###  http://www.semanticweb.org/ivans/ontologies/2025/dt-code-generation/PropertyChangeByActuation
:PropertyChangeByActuation rdf:type owl:Class ;
                           rdfs:subClassOf :PropertyChange ,
                                           [ rdf:type owl:Restriction ;
                                             owl:onProperty :enactedBy ;
                                             owl:minQualifiedCardinality "1"^^xsd:nonNegativeInteger ;
                                             owl:onClass :ActuatorState
                                           ] ;
                           owl:disjointWith :PropertyChangeByReconfiguration ;
                           rdfs:comment "Represents a specific PropertyChange as a result of actuating on the respective Property."@en ;
                           rdfs:label "PropertyChangeByActuation"@en .


###  http://www.semanticweb.org/ivans/ontologies/2025/dt-code-generation/PropertyChangeByReconfiguration
:PropertyChangeByReconfiguration rdf:type owl:Class ;
                                 rdfs:subClassOf :PropertyChange ,
                                                 [ rdf:type owl:Restriction ;
                                                   owl:onProperty :enactedBy ;
                                                   owl:minQualifiedCardinality "1"^^xsd:nonNegativeInteger ;
                                                   owl:onClass :ConfigurableParameter
                                                 ] ,
                                                 [ rdf:type owl:Restriction ;
                                                   owl:onProperty :alteredBy ;
                                                   owl:qualifiedCardinality "1"^^xsd:nonNegativeInteger ;
                                                   owl:onClass :Effect
                                                 ] ;
                                 rdfs:comment "Represents a specific PropertyChange as a result of reconfiguring a related ConfigurableProperty."@en ;
                                 rdfs:label "PropertyChangeByReconfiguration"@en .


###  http://www.semanticweb.org/ivans/ontologies/2025/dt-code-generation/ReconfigurationAction
:ReconfigurationAction rdf:type owl:Class ;
                       rdfs:subClassOf :Action ,
                                       [ rdf:type owl:Restriction ;
                                         owl:onProperty :affectsPropertyWith ;
                                         owl:qualifiedCardinality "1"^^xsd:nonNegativeInteger ;
                                         owl:onClass :Effect
                                       ] ,
                                       [ rdf:type owl:Restriction ;
                                         owl:onProperty <http://www.w3.org/ns/ssn/forProperty> ;
                                         owl:qualifiedCardinality "1"^^xsd:nonNegativeInteger ;
                                         owl:onClass :ConfigurableParameter
                                       ] ,
                                       [ rdf:type owl:Restriction ;
                                         owl:onProperty :altersBy ;
                                         owl:cardinality "1"^^xsd:nonNegativeInteger
                                       ] ;
                       rdfs:comment "Represents a single system Action with a parameter reconfiguration, either for optimization or regaining optimal conditions."@en ;
                       rdfs:label "ReconfigurationAction"@en .


###  http://www.w3.org/ns/sosa/Actuator
<http://www.w3.org/ns/sosa/Actuator> rdfs:subClassOf [ rdf:type owl:Restriction ;
                                                       owl:onProperty :hasActuatorState ;
                                                       owl:minQualifiedCardinality "1"^^xsd:nonNegativeInteger ;
                                                       owl:onClass :ActuatorState
                                                     ] .


###  http://www.w3.org/ns/sosa/ObservableProperty
<http://www.w3.org/ns/sosa/ObservableProperty> rdfs:subClassOf [ rdf:type owl:Restriction ;
                                                                 owl:onProperty :hasValue ;
                                                                 owl:cardinality "1"^^xsd:nonNegativeInteger
                                                               ] .


###  http://www.w3.org/ns/sosa/Platform
<http://www.w3.org/ns/sosa/Platform> rdfs:subClassOf [ rdf:type owl:Restriction ;
                                                       owl:onProperty :optimizesFor ;
                                                       owl:minQualifiedCardinality "1"^^xsd:nonNegativeInteger ;
                                                       owl:onClass :PropertyChange
                                                     ] ,
                                                     [ rdf:type owl:Restriction ;
                                                       owl:onProperty <http://www.w3.org/ns/ssn/implements> ;
                                                       owl:minQualifiedCardinality "1"^^xsd:nonNegativeInteger ;
                                                       owl:onClass :OptimalCondition
                                                     ] .


###  http://www.w3.org/ns/ssn/Input
<http://www.w3.org/ns/ssn/Input> rdfs:subClassOf <http://www.w3.org/ns/ssn/Property> ,
                                                 [ rdf:type owl:Restriction ;
                                                   owl:onProperty :hasValue ;
                                                   owl:cardinality "1"^^xsd:nonNegativeInteger
                                                 ] .


###  http://www.w3.org/ns/ssn/Output
<http://www.w3.org/ns/ssn/Output> rdfs:subClassOf <http://www.w3.org/ns/ssn/Property> ,
                                                  [ rdf:type owl:Restriction ;
                                                    owl:onProperty :hasValue ;
                                                    owl:cardinality "1"^^xsd:nonNegativeInteger
                                                  ] .


#################################################################
#    Individuals
#################################################################

###  http://www.semanticweb.org/ivans/ontologies/2025/dt-code-generation/ValueDecrease
:ValueDecrease rdf:type owl:NamedIndividual ,
                        :Effect .


###  http://www.semanticweb.org/ivans/ontologies/2025/dt-code-generation/ValueIncrease
:ValueIncrease rdf:type owl:NamedIndividual ,
                        :Effect .


###  Generated by the OWL API (version 4.5.29.2024-05-13T12:11:03Z) https://github.com/owlcs/owlapi
