@prefix : <http://www.semanticweb.org/ivans/ontologies/2025/ruleless-digital-twins/> .
@prefix owl: <http://www.w3.org/2002/07/owl#> .
@prefix rdf: <http://www.w3.org/1999/02/22-rdf-syntax-ns#> .
@prefix xml: <http://www.w3.org/XML/1998/namespace> .
@prefix xsd: <http://www.w3.org/2001/XMLSchema#> .
@prefix rdfs: <http://www.w3.org/2000/01/rdf-schema#> .
@base <http://www.semanticweb.org/ivans/ontologies/2025/ruleless-digital-twins/> .

<http://www.semanticweb.org/ivans/ontologies/2025/ruleless-digital-twins> rdf:type owl:Ontology ;
                                                                           owl:imports <http://www.w3.org/ns/ssn/> .

#################################################################
#    Datatypes
#################################################################

###  http://www.w3.org/2001/XMLSchema#duration
xsd:duration rdf:type rdfs:Datatype .


#################################################################
#    Object Properties
#################################################################

###  http://www.semanticweb.org/ivans/ontologies/2025/ruleless-digital-twins/affectsPropertyWith
:affectsPropertyWith rdf:type owl:ObjectProperty ;
                     rdfs:range :Effect ;
                     rdfs:comment "Represents that a Thing has an effect on a Property."@en ;
                     rdfs:label "affectsPropertyWith"@en .


###  http://www.semanticweb.org/ivans/ontologies/2025/ruleless-digital-twins/alteredBy
:alteredBy rdf:type owl:ObjectProperty ;
           rdfs:domain :PropertyChangeByReconfiguration ;
           rdfs:range :Effect ;
           rdfs:comment "Represents a relation between a ConfigurableProperty and an Effect on it that causes a related property to change."@en ;
           rdfs:label "alteredBy"@en .


###  http://www.semanticweb.org/ivans/ontologies/2025/ruleless-digital-twins/arithmeticOperator
:arithmeticOperator rdf:type owl:ObjectProperty ;
                    rdfs:subPropertyOf :operator .


###  http://www.semanticweb.org/ivans/ontologies/2025/ruleless-digital-twins/comparisonOperator
:comparisonOperator rdf:type owl:ObjectProperty ;
                    rdfs:subPropertyOf :operator ;
                    rdfs:domain :Constraint ;
                    rdfs:range <http://www.w3.org/ns/ssn/Property> ;
                    rdfs:comment "Required to enable Condition constraints on variable Property values. Since it is not possible to use the standard comparison operators (>, <, >=, <=) on non-literals, this property allows us to do so."@en ;
                    rdfs:label "comparisonOperator"@en .


###  http://www.semanticweb.org/ivans/ontologies/2025/ruleless-digital-twins/enactedBy
:enactedBy rdf:type owl:ObjectProperty ;
           owl:inverseOf :enacts ;
           rdfs:comment "Represents a relation between a PropertyChange and a thing, such as a System or Actuator."@en ;
           rdfs:label "enactedBy"@en .


###  http://www.semanticweb.org/ivans/ontologies/2025/ruleless-digital-twins/enacts
:enacts rdf:type owl:ObjectProperty ;
        rdfs:range :PropertyChange ;
        rdfs:comment "Represents a relation between a thing, such as a System or Actuator, and a PropertyChange."@en ;
        rdfs:label "enacts"@en .


###  http://www.semanticweb.org/ivans/ontologies/2025/ruleless-digital-twins/equalTo
:equalTo rdf:type owl:ObjectProperty ;
         rdfs:subPropertyOf :comparisonOperator ;
         rdfs:comment "Represents the '=' (equal to) comparison operator for Property-based values."@en ;
         rdfs:label "equalTo"@en .


###  http://www.semanticweb.org/ivans/ontologies/2025/ruleless-digital-twins/greaterThan
:greaterThan rdf:type owl:ObjectProperty ;
             rdfs:subPropertyOf :comparisonOperator ;
             rdfs:comment "Represents the '>' (greater than) comparison operator for Property-based values."@en ;
             rdfs:label "greaterThan"@en .


###  http://www.semanticweb.org/ivans/ontologies/2025/ruleless-digital-twins/greaterThanOrEqualTo
:greaterThanOrEqualTo rdf:type owl:ObjectProperty ;
                      rdfs:subPropertyOf :comparisonOperator ;
                      rdfs:comment "Represents the '>=' (greater than or equal to) comparison operator for Property-based values."@en ;
                      rdfs:label "greaterThanOrEqualTo"@en .


###  http://www.semanticweb.org/ivans/ontologies/2025/ruleless-digital-twins/hasActuator
:hasActuator rdf:type owl:ObjectProperty ;
             rdfs:domain :ActuationAction ;
             rdfs:range <http://www.w3.org/ns/sosa/Actuator> ;
             rdfs:comment "The relation between an ActuationExecution and an Actuator it uses."@en ;
             rdfs:label "hasActuator"@en .


###  http://www.semanticweb.org/ivans/ontologies/2025/ruleless-digital-twins/hasConstraint
:hasConstraint rdf:type owl:ObjectProperty ;
               rdfs:domain :Condition ;
               rdfs:range :Constraint ;
               rdfs:comment "Represents a relation between a Condition and a Constraint."@en ;
               rdfs:label "hasConstraint"@en .


###  http://www.semanticweb.org/ivans/ontologies/2025/ruleless-digital-twins/hasSimulationModel
:hasSimulationModel rdf:type owl:ObjectProperty ;
                    rdfs:domain <http://www.w3.org/ns/sosa/Platform> ;
                    rdfs:range <http://www.w3.org/ns/sosa/Procedure> ;
                    rdfs:comment "Represents a model used for simulations of the corresponding Platform."@en ;
                    rdfs:label "hasSimulationModel"@en .


###  http://www.semanticweb.org/ivans/ontologies/2025/ruleless-digital-twins/isInputOf
:isInputOf rdf:type owl:ObjectProperty ;
           owl:inverseOf <http://www.w3.org/ns/ssn/hasInput> ;
           rdfs:comment "Relation between an Input and its Procedure."@en ;
           rdfs:label "isInputOf"@en .


###  http://www.semanticweb.org/ivans/ontologies/2025/ruleless-digital-twins/isOutputOf
:isOutputOf rdf:type owl:ObjectProperty ;
            owl:inverseOf <http://www.w3.org/ns/ssn/hasOutput> ;
            rdfs:comment "Relation between an Output and its Procedure."@en ;
            rdfs:label "isOutputOf"@en .


###  http://www.semanticweb.org/ivans/ontologies/2025/ruleless-digital-twins/lessThan
:lessThan rdf:type owl:ObjectProperty ;
          rdfs:subPropertyOf :comparisonOperator ;
          rdfs:comment "Represents the '<' (less than) comparison operator for Property-based values."@en ;
          rdfs:label "lessThan"@en .


###  http://www.semanticweb.org/ivans/ontologies/2025/ruleless-digital-twins/lessThanOrEqualTo
:lessThanOrEqualTo rdf:type owl:ObjectProperty ;
                   rdfs:subPropertyOf :comparisonOperator ;
                   rdfs:comment "Represents the '<=' (less than or equal to) comparison operator for Property-based values."@en ;
                   rdfs:label "lessThanOrEqualTo"@en .


###  http://www.semanticweb.org/ivans/ontologies/2025/ruleless-digital-twins/minus
:minus rdf:type owl:ObjectProperty ;
       rdfs:subPropertyOf :arithmeticOperator ;
       rdfs:comment "Represents the '-' (subtraction) arithmetic operator for Property-based values."@en ;
       rdfs:label "minus"@en .


###  http://www.semanticweb.org/ivans/ontologies/2025/ruleless-digital-twins/operator
:operator rdf:type owl:ObjectProperty ;
          rdfs:range <http://www.w3.org/ns/ssn/Property> ;
          rdfs:comment "Represents an operator property that can be used on non-literals. Decidability terms and conditions apply."@en ;
          rdfs:label "operator"@en .


###  http://www.semanticweb.org/ivans/ontologies/2025/ruleless-digital-twins/optimizedBy
:optimizedBy rdf:type owl:ObjectProperty ;
             owl:inverseOf :optimizesFor ;
             rdfs:comment "A relation between a Property and a Platform optimizing for it."@en ;
             rdfs:label "optimizedBy"@en .


###  http://www.semanticweb.org/ivans/ontologies/2025/ruleless-digital-twins/optimizesFor
:optimizesFor rdf:type owl:ObjectProperty ;
              rdfs:domain <http://www.w3.org/ns/sosa/Platform> ;
              rdfs:range :PropertyChange ;
              rdfs:comment "Represents a relation between a platform and a PropertyChange that indicates that platform's optimization of those properties."@en ;
              rdfs:label "optimizesFor"@en .


###  http://www.semanticweb.org/ivans/ontologies/2025/ruleless-digital-twins/over
:over rdf:type owl:ObjectProperty ;
      rdfs:subPropertyOf :arithmeticOperator ;
      rdfs:comment "Represents the '/' (division) arithmetic operator for Property-based values."@en ;
      rdfs:label "over"@en .


###  http://www.semanticweb.org/ivans/ontologies/2025/ruleless-digital-twins/plus
:plus rdf:type owl:ObjectProperty ;
      rdfs:subPropertyOf :arithmeticOperator ;
      rdfs:comment "Represents the '+' (addition) arithmetic operator for Property-based values."@en ;
      rdfs:label "plus"@en .


###  http://www.semanticweb.org/ivans/ontologies/2025/ruleless-digital-twins/propertyFor
:propertyFor rdf:type owl:ObjectProperty ;
             owl:inverseOf <http://www.w3.org/ns/ssn/forProperty> ;
             rdfs:comment "A relation between some property and an entity."@en ;
             rdfs:label "property for"@en .


###  http://www.semanticweb.org/ivans/ontologies/2025/ruleless-digital-twins/times
:times rdf:type owl:ObjectProperty ;
       rdfs:subPropertyOf :arithmeticOperator ;
       rdfs:comment "Represents the '*' (multiplication) arithmetic operator for Property-based values."@en ;
       rdfs:label "times"@en .


#################################################################
#    Data properties
#################################################################

###  http://www.semanticweb.org/ivans/ontologies/2025/ruleless-digital-twins/generateCombinationsOnlyFromOptimalConditions
:generateCombinationsOnlyFromOptimalConditions rdf:type owl:DatatypeProperty ;
                                               rdfs:domain <http://www.w3.org/ns/sosa/Platform> ;
                                               rdfs:range xsd:boolean ;
                                               rdfs:comment "Determines how ActionCombination generation for a Platforms future simulations occurs. 'false' generates all possible combinations from all actuators and their states in the instance model. 'true' restricts combination generation to only the relevant actuators and their states that potentially restore violated OptimalConditions."@en ;
                                               rdfs:label "generateCombinationsOnlyFromOptimalConditions"@en .


###  http://www.semanticweb.org/ivans/ontologies/2025/ruleless-digital-twins/hasActuatorState
:hasActuatorState rdf:type owl:DatatypeProperty ;
                  rdfs:domain [ rdf:type owl:Class ;
                                owl:unionOf ( :ActuationAction
                                              <http://www.w3.org/ns/sosa/Actuator>
                                            )
                              ] ;
                  rdfs:range rdfs:Literal ;
                  rdfs:comment "Represents a relation between an Actuator and its state."@en ;
                  rdfs:label "hasActuatorState"@en .


###  http://www.semanticweb.org/ivans/ontologies/2025/ruleless-digital-twins/hasIdentifier
:hasIdentifier rdf:type owl:DatatypeProperty ;
               rdfs:range xsd:string ;
               rdfs:comment "Represents a relation from a thing to its identifier."@en ;
               rdfs:label "hasIdentifier"@en .


###  http://www.semanticweb.org/ivans/ontologies/2025/ruleless-digital-twins/hasPossibleValue
:hasPossibleValue rdf:type owl:DatatypeProperty ;
                  rdfs:domain :ConfigurableParameter ;
                  rdfs:range rdfs:Literal ;
                  rdfs:comment "Represents one value that a ConfigurableParameter can have."@en ;
                  rdfs:label "hasPossibleValue"@en .


###  http://www.semanticweb.org/ivans/ontologies/2025/ruleless-digital-twins/hasPriority
:hasPriority rdf:type owl:DatatypeProperty ;
             rdfs:domain :OptimalCondition ;
             rdfs:range xsd:int ;
             rdfs:comment "Classifies an OptimalCondition as having a specific priority to facilitate DT decision making by ranking."@en ;
             rdfs:label "hasPriority"@en .


###  http://www.semanticweb.org/ivans/ontologies/2025/ruleless-digital-twins/hasSimulationFidelitySeconds
:hasSimulationFidelitySeconds rdf:type owl:DatatypeProperty ;
                              rdfs:domain :FmuModel ;
                              rdfs:range xsd:int ;
                              rdfs:comment "Represents the fidelity of the simulation models (FMUs) with respect to the equations they contain."@en ;
                              rdfs:label "hasSimulationFidelitySeconds"@en .


###  http://www.semanticweb.org/ivans/ontologies/2025/ruleless-digital-twins/hasTimeLimit
:hasTimeLimit rdf:type owl:DatatypeProperty ;
              rdfs:range xsd:duration ;
              rdfs:comment "Represents a time limit on the duration of the Strategy."@en ;
              rdfs:label "hasTimeLimit"@en .


###  http://www.semanticweb.org/ivans/ontologies/2025/ruleless-digital-twins/hasURI
:hasURI rdf:type owl:DatatypeProperty ;
        rdfs:domain :FmuModel ;
        rdfs:range xsd:anyURI ;
        rdfs:comment "Refers to an FMUs URI."@en ;
        rdfs:label "hasURI"@en .


###  http://www.semanticweb.org/ivans/ontologies/2025/ruleless-digital-twins/hasValue
:hasValue rdf:type owl:DatatypeProperty ;
          rdfs:range rdfs:Literal ;
          rdfs:comment "Describes a relation to a specific value (of a specific type) contained by a property or an Input/Output parameter."@en ;
          rdfs:label "hasValue"@en .


###  http://www.semanticweb.org/ivans/ontologies/2025/ruleless-digital-twins/reachedInMaximumSeconds
:reachedInMaximumSeconds rdf:type owl:DatatypeProperty ;
                         rdfs:domain :Condition ;
                         rdfs:range xsd:int ;
                         rdfs:comment "Represents the maximum amount of time in seconds to reach an OptimalCondition."@en ;
                         rdfs:label "reachedInMaximumSeconds"@en .


###  http://www.semanticweb.org/ivans/ontologies/2025/ruleless-digital-twins/satisfiedBy
:satisfiedBy rdf:type owl:DatatypeProperty ;
             rdfs:domain :Condition ;
             rdfs:range xsd:dateTimeStamp ;
             rdfs:comment "Represents a relation between a Condition and the time that Condition must be satisfied at. In case of no specified time, the Condition should always be satisfied."@en ;
             rdfs:label "satisfiedBy"@en .


#################################################################
#    Classes
#################################################################

###  http://www.semanticweb.org/ivans/ontologies/2025/ruleless-digital-twins/Action
:Action rdf:type owl:Class ;
        rdfs:comment "Represents a single system Action."@en ;
        rdfs:label "Action"@en .


###  http://www.semanticweb.org/ivans/ontologies/2025/ruleless-digital-twins/ActionCombination
:ActionCombination rdf:type owl:Class ;
                   rdfs:comment "Acts as a wrapper for multiple Actions."@en ;
                   rdfs:label "ActionCombination"@en .


###  http://www.semanticweb.org/ivans/ontologies/2025/ruleless-digital-twins/ActuationAction
:ActuationAction rdf:type owl:Class ;
                 rdfs:subClassOf :Action ,
                                 [ rdf:type owl:Restriction ;
                                   owl:onProperty :hasActuator ;
                                   owl:qualifiedCardinality "1"^^xsd:nonNegativeInteger ;
                                   owl:onClass <http://www.w3.org/ns/sosa/Actuator>
                                 ] ,
                                 [ rdf:type owl:Restriction ;
                                   owl:onProperty :hasActuatorState ;
                                   owl:cardinality "1"^^xsd:nonNegativeInteger
                                 ] ;
                 owl:disjointWith :ReconfigurationAction ;
                 rdfs:comment "Represents a single system Action with an actuation, either for optimization or regaining optimal conditions."@en ;
                 rdfs:label "ActuationAction"@en .


###  http://www.semanticweb.org/ivans/ontologies/2025/ruleless-digital-twins/Condition
:Condition rdf:type owl:Class ;
           rdfs:subClassOf [ rdf:type owl:Restriction ;
                             owl:onProperty <http://www.w3.org/ns/ssn/forProperty> ;
                             owl:qualifiedCardinality "1"^^xsd:nonNegativeInteger ;
                             owl:onClass <http://www.w3.org/ns/ssn/Property>
                           ] ,
                           [ rdf:type owl:Restriction ;
                             owl:onProperty :satisfiedBy ;
                             owl:someValuesFrom xsd:dateTimeStamp
                           ] ,
                           [ rdf:type owl:Restriction ;
                             owl:onProperty :hasPriority ;
                             owl:maxQualifiedCardinality "1"^^xsd:nonNegativeInteger ;
                             owl:onDataRange xsd:int
                           ] ,
                           [ rdf:type owl:Restriction ;
                             owl:onProperty :reachedInMaximumSeconds ;
                             owl:maxQualifiedCardinality "1"^^xsd:nonNegativeInteger ;
                             owl:onDataRange xsd:int
                           ] ;
           rdfs:comment "Represents a required value range constraint on a Property.  For example, a condition on the temperature of a room could be defined as values greater than 18 and lower than 22 degrees Celsius."@en ;
           rdfs:label "Condition"@en .


###  http://www.semanticweb.org/ivans/ontologies/2025/ruleless-digital-twins/ConfigurableParameter
:ConfigurableParameter rdf:type owl:Class ;
                       rdfs:subClassOf <http://www.w3.org/ns/ssn/Input> ,
                                       <http://www.w3.org/ns/ssn/Property> ,
                                       [ rdf:type owl:Restriction ;
                                         owl:onProperty :enacts ;
                                         owl:minQualifiedCardinality "1"^^xsd:nonNegativeInteger ;
                                         owl:onClass :PropertyChangeByReconfiguration
                                       ] ,
                                       [ rdf:type owl:Restriction ;
                                         owl:onProperty :hasValue ;
                                         owl:minCardinality "1"^^xsd:nonNegativeInteger
                                       ] ;
                       rdfs:comment "A parameter not directly observable or actuatable but rather used for configuring an an Input to a System or Procedure."@en ;
                       rdfs:label "ConfigurableParameter"@en .


###  http://www.semanticweb.org/ivans/ontologies/2025/ruleless-digital-twins/Constraint
:Constraint rdf:type owl:Class ;
            rdfs:subClassOf [ rdf:type owl:Class ;
                              owl:unionOf ( [ rdf:type owl:Restriction ;
                                              owl:onProperty :greaterThan ;
                                              owl:qualifiedCardinality "1"^^xsd:nonNegativeInteger ;
                                              owl:onClass <http://www.w3.org/ns/ssn/Property>
                                            ]
                                            [ rdf:type owl:Restriction ;
                                              owl:onProperty :greaterThanOrEqualTo ;
                                              owl:qualifiedCardinality "1"^^xsd:nonNegativeInteger ;
                                              owl:onClass <http://www.w3.org/ns/ssn/Property>
                                            ]
                                          )
                            ] ;
            rdfs:comment "Represents a value constraint used by Conditions."@en ;
            rdfs:label "Constraint"@en .


###  http://www.semanticweb.org/ivans/ontologies/2025/ruleless-digital-twins/Effect
:Effect rdf:type owl:Class ;
        rdfs:comment "The type of effect on the value of a property."@en ;
        rdfs:label "Effect"@en .


###  http://www.semanticweb.org/ivans/ontologies/2025/ruleless-digital-twins/FmuModel
:FmuModel rdf:type owl:Class ;
          rdfs:subClassOf <http://www.w3.org/ns/sosa/Procedure> ,
                          [ rdf:type owl:Restriction ;
                            owl:onProperty :hasSimulationFidelitySeconds ;
                            owl:qualifiedCardinality "1"^^xsd:nonNegativeInteger ;
                            owl:onDataRange xsd:int
                          ] ,
                          [ rdf:type owl:Restriction ;
                            owl:onProperty :hasURI ;
                            owl:qualifiedCardinality "1"^^xsd:nonNegativeInteger ;
                            owl:onDataRange xsd:anyURI
                          ] ;
          rdfs:comment "Represents a simulation model in the form of a Functional Mock-up Unit (FMU)."@en ;
          rdfs:label "FmuModel"@en .


###  http://www.semanticweb.org/ivans/ontologies/2025/ruleless-digital-twins/OptimalCondition
:OptimalCondition rdf:type owl:Class ;
                  rdfs:subClassOf :Condition ;
                  rdfs:comment "Represents a softer Condition that may be broken for the purposes of achieving a more optimal long-term DT decision."@en ;
                  rdfs:label "OptimalCondition"@en .


###  http://www.semanticweb.org/ivans/ontologies/2025/ruleless-digital-twins/PropertyChange
:PropertyChange rdf:type owl:Class ;
                rdfs:subClassOf [ rdf:type owl:Restriction ;
                                  owl:onProperty :affectsPropertyWith ;
                                  owl:qualifiedCardinality "1"^^xsd:nonNegativeInteger ;
                                  owl:onClass :Effect
                                ] ,
                                [ rdf:type owl:Restriction ;
                                  owl:onProperty <http://www.w3.org/ns/ssn/forProperty> ;
                                  owl:qualifiedCardinality "1"^^xsd:nonNegativeInteger ;
                                  owl:onClass <http://www.w3.org/ns/ssn/Property>
                                ] ;
                rdfs:comment "Represents a specific property change in a given system, either via a changed configuration property or an actuation on an observable one."@en ;
                rdfs:label "PropertyChange"@en .


###  http://www.semanticweb.org/ivans/ontologies/2025/ruleless-digital-twins/PropertyChangeByActuation
:PropertyChangeByActuation rdf:type owl:Class ;
                           rdfs:subClassOf :PropertyChange ,
                                           [ rdf:type owl:Restriction ;
                                             owl:onProperty :enactedBy ;
                                             owl:minQualifiedCardinality "1"^^xsd:nonNegativeInteger ;
                                             owl:onClass <http://www.w3.org/ns/sosa/Actuator>
                                           ] ;
                           owl:disjointWith :PropertyChangeByReconfiguration ;
                           rdfs:comment "Represents a specific PropertyChange as a result of actuating on the respective Property."@en ;
                           rdfs:label "PropertyChangeByActuation"@en .


###  http://www.semanticweb.org/ivans/ontologies/2025/ruleless-digital-twins/PropertyChangeByReconfiguration
:PropertyChangeByReconfiguration rdf:type owl:Class ;
                                 rdfs:subClassOf :PropertyChange ,
                                                 [ rdf:type owl:Restriction ;
                                                   owl:onProperty :enactedBy ;
                                                   owl:minQualifiedCardinality "1"^^xsd:nonNegativeInteger ;
                                                   owl:onClass :ConfigurableParameter
                                                 ] ,
                                                 [ rdf:type owl:Restriction ;
                                                   owl:onProperty :alteredBy ;
                                                   owl:qualifiedCardinality "1"^^xsd:nonNegativeInteger ;
                                                   owl:onClass :Effect
                                                 ] ;
                                 rdfs:comment "Represents a specific PropertyChange as a result of reconfiguring a related ConfigurableProperty."@en ;
                                 rdfs:label "PropertyChangeByReconfiguration"@en .


###  http://www.semanticweb.org/ivans/ontologies/2025/ruleless-digital-twins/ReconfigurationAction
:ReconfigurationAction rdf:type owl:Class ;
                       rdfs:subClassOf :Action ,
                                       [ rdf:type owl:Restriction ;
                                         owl:onProperty <http://www.w3.org/ns/ssn/forProperty> ;
                                         owl:qualifiedCardinality "1"^^xsd:nonNegativeInteger ;
                                         owl:onClass :ConfigurableParameter
                                       ] ,
                                       [ rdf:type owl:Restriction ;
                                         owl:onProperty :hasValue ;
                                         owl:cardinality "1"^^xsd:nonNegativeInteger
                                       ] ;
                       rdfs:comment "Represents a single system Action with a parameter reconfiguration, either for optimization or regaining optimal conditions."@en ;
                       rdfs:label "ReconfigurationAction"@en .


###  http://www.w3.org/ns/sosa/Actuator
<http://www.w3.org/ns/sosa/Actuator> rdfs:subClassOf [ rdf:type owl:Restriction ;
                                                       owl:onProperty :enacts ;
                                                       owl:minQualifiedCardinality "1"^^xsd:nonNegativeInteger ;
                                                       owl:onClass :PropertyChangeByActuation
                                                     ] ,
                                                     [ rdf:type owl:Restriction ;
                                                       owl:onProperty :hasActuatorState ;
                                                       owl:minCardinality "1"^^xsd:nonNegativeInteger
                                                     ] .


###  http://www.w3.org/ns/sosa/ObservableProperty
<http://www.w3.org/ns/sosa/ObservableProperty> rdfs:subClassOf [ rdf:type owl:Restriction ;
                                                                 owl:onProperty :hasValue ;
                                                                 owl:cardinality "1"^^xsd:nonNegativeInteger
                                                               ] .


###  http://www.w3.org/ns/sosa/Platform
<http://www.w3.org/ns/sosa/Platform> rdfs:subClassOf [ rdf:type owl:Restriction ;
                                                       owl:onProperty :optimizesFor ;
                                                       owl:minQualifiedCardinality "1"^^xsd:nonNegativeInteger ;
                                                       owl:onClass :PropertyChange
                                                     ] ,
                                                     [ rdf:type owl:Restriction ;
                                                       owl:onProperty <http://www.w3.org/ns/ssn/implements> ;
                                                       owl:minQualifiedCardinality "1"^^xsd:nonNegativeInteger ;
                                                       owl:onClass :OptimalCondition
                                                     ] ,
                                                     [ rdf:type owl:Restriction ;
                                                       owl:onProperty :hasSimulationModel ;
                                                       owl:qualifiedCardinality "1"^^xsd:nonNegativeInteger ;
                                                       owl:onClass :FmuModel
                                                     ] ,
                                                     [ rdf:type owl:Restriction ;
                                                       owl:onProperty :generateCombinationsOnlyFromOptimalConditions ;
                                                       owl:qualifiedCardinality "1"^^xsd:nonNegativeInteger ;
                                                       owl:onDataRange xsd:boolean
                                                     ] .


#################################################################
#    Individuals
#################################################################

###  http://www.semanticweb.org/ivans/ontologies/2025/ruleless-digital-twins/ValueDecrease
:ValueDecrease rdf:type owl:NamedIndividual ,
                        :Effect .


###  http://www.semanticweb.org/ivans/ontologies/2025/ruleless-digital-twins/ValueIncrease
:ValueIncrease rdf:type owl:NamedIndividual ,
                        :Effect .


###  http://www.semanticweb.org/ivans/ontologies/2025/ruleless-digital-twins/test
:test rdf:type owl:NamedIndividual ,
               :Constraint ,
               [ rdf:type owl:Restriction ;
                 owl:onProperty :equalTo ;
                 owl:hasValue :testprop2
               ] .


###  http://www.semanticweb.org/ivans/ontologies/2025/ruleless-digital-twins/testprop1
:testprop1 rdf:type owl:NamedIndividual ,
                    <http://www.w3.org/ns/ssn/Property> ;
           owl:differentFrom :testprop2 .


###  http://www.semanticweb.org/ivans/ontologies/2025/ruleless-digital-twins/testprop2
:testprop2 rdf:type owl:NamedIndividual ,
                    <http://www.w3.org/ns/ssn/Property> .


###  Generated by the OWL API (version 4.5.29.2024-05-13T12:11:03Z) https://github.com/owlcs/owlapi
