@prefix : <http://www.semanticweb.org/ivans/ontologies/2025/ruleless-digital-twins/> .
@prefix owl: <http://www.w3.org/2002/07/owl#> .
@prefix rdf: <http://www.w3.org/1999/02/22-rdf-syntax-ns#> .
@prefix xml: <http://www.w3.org/XML/1998/namespace> .
@prefix xsd: <http://www.w3.org/2001/XMLSchema#> .
@prefix rdfs: <http://www.w3.org/2000/01/rdf-schema#> .
@base <http://www.semanticweb.org/ivans/ontologies/2025/ruleless-digital-twins/> .

<http://www.semanticweb.org/ivans/ontologies/2025/ruleless-digital-twins> rdf:type owl:Ontology ;
                                                                           owl:imports <http://www.w3.org/ns/ssn/> .

#################################################################
#    Datatypes
#################################################################

###  http://www.w3.org/2001/XMLSchema#duration
xsd:duration rdf:type rdfs:Datatype .


#################################################################
#    Object Properties
#################################################################

###  http://www.semanticweb.org/ivans/ontologies/2025/ruleless-digital-twins/affectsPropertyWith
:affectsPropertyWith rdf:type owl:ObjectProperty ;
                     rdfs:range :Effect ;
                     rdfs:comment "Represents that a Thing has an effect on a Property."@en ;
                     rdfs:label "affectsPropertyWith"@en .


###  http://www.semanticweb.org/ivans/ontologies/2025/ruleless-digital-twins/alteredBy
:alteredBy rdf:type owl:ObjectProperty ;
           rdfs:domain :PropertyChangeByReconfiguration ;
           rdfs:range :Effect ;
           rdfs:comment "Represents a relation between a ConfigurableProperty and an Effect on it that causes a related property to change."@en ;
           rdfs:label "alteredBy"@en .


###  http://www.semanticweb.org/ivans/ontologies/2025/ruleless-digital-twins/enactedBy
:enactedBy rdf:type owl:ObjectProperty ;
           owl:inverseOf :enacts ;
           rdfs:comment "Represents a relation between a PropertyChange and a thing, such as a System or Actuator."@en ;
           rdfs:label "enactedBy"@en .


###  http://www.semanticweb.org/ivans/ontologies/2025/ruleless-digital-twins/enacts
:enacts rdf:type owl:ObjectProperty ;
        rdfs:range :PropertyChange ;
        rdfs:comment "Represents a relation between a thing, such as a System or Actuator, and a PropertyChange."@en ;
        rdfs:label "enacts"@en .


###  http://www.semanticweb.org/ivans/ontologies/2025/ruleless-digital-twins/hasActionValueGenerator
:hasActionValueGenerator rdf:type owl:ObjectProperty ;
                         rdfs:range :ActionValueGenerator .


###  http://www.semanticweb.org/ivans/ontologies/2025/ruleless-digital-twins/hasActuationValueGenerator
:hasActuationValueGenerator rdf:type owl:ObjectProperty ;
                            rdfs:subPropertyOf :hasActionValueGenerator ;
                            rdfs:domain <http://www.w3.org/ns/sosa/Actuator> ;
                            rdfs:range :ActuationValueGenerator .


###  http://www.semanticweb.org/ivans/ontologies/2025/ruleless-digital-twins/hasActuator
:hasActuator rdf:type owl:ObjectProperty ;
             rdfs:domain :ActuationAction ;
             rdfs:range <http://www.w3.org/ns/sosa/Actuator> ;
             rdfs:comment "The relation between an ActuationExecution and an Actuator it uses."@en ;
             rdfs:label "hasActuator"@en .


###  http://www.semanticweb.org/ivans/ontologies/2025/ruleless-digital-twins/hasReconfigurationValueGenerator
:hasReconfigurationValueGenerator rdf:type owl:ObjectProperty ;
                                  rdfs:subPropertyOf :hasActionValueGenerator ;
                                  rdfs:domain :ConfigurableParameter ;
                                  rdfs:range :ReconfigurationValueGenerator .


###  http://www.semanticweb.org/ivans/ontologies/2025/ruleless-digital-twins/hasSimulationModel
:hasSimulationModel rdf:type owl:ObjectProperty ;
                    rdfs:domain <http://www.w3.org/ns/sosa/Platform> ;
                    rdfs:range <http://www.w3.org/ns/sosa/Procedure> ;
                    rdfs:comment "Represents a model used for simulations of the corresponding Platform."@en ;
                    rdfs:label "hasSimulationModel"@en .


###  http://www.semanticweb.org/ivans/ontologies/2025/ruleless-digital-twins/isInputOf
:isInputOf rdf:type owl:ObjectProperty ;
           owl:inverseOf <http://www.w3.org/ns/ssn/hasInput> ;
           rdfs:comment "Relation between an Input and its Procedure."@en ;
           rdfs:label "isInputOf"@en .


###  http://www.semanticweb.org/ivans/ontologies/2025/ruleless-digital-twins/isOutputOf
:isOutputOf rdf:type owl:ObjectProperty ;
            owl:inverseOf <http://www.w3.org/ns/ssn/hasOutput> ;
            rdfs:comment "Relation between an Output and its Procedure."@en ;
            rdfs:label "isOutputOf"@en .


###  http://www.semanticweb.org/ivans/ontologies/2025/ruleless-digital-twins/optimizedBy
:optimizedBy rdf:type owl:ObjectProperty ;
             owl:inverseOf :optimizesFor ;
             rdfs:comment "A relation between a Property and a Platform optimizing for it."@en ;
             rdfs:label "optimizedBy"@en .


###  http://www.semanticweb.org/ivans/ontologies/2025/ruleless-digital-twins/optimizesFor
:optimizesFor rdf:type owl:ObjectProperty ;
              rdfs:domain <http://www.w3.org/ns/sosa/Platform> ;
              rdfs:range :PropertyChange ;
              rdfs:comment "Represents a relation between a platform and a PropertyChange that indicates that platform's optimization of those properties."@en ;
              rdfs:label "optimizesFor"@en .


###  http://www.semanticweb.org/ivans/ontologies/2025/ruleless-digital-twins/propertyFor
:propertyFor rdf:type owl:ObjectProperty ;
             owl:inverseOf <http://www.w3.org/ns/ssn/forProperty> ;
             rdfs:comment "A relation between some property and an entity."@en ;
             rdfs:label "property for"@en .


#################################################################
#    Data properties
#################################################################

###  http://www.semanticweb.org/ivans/ontologies/2025/ruleless-digital-twins/configuresNewValue
:configuresNewValue rdf:type owl:DatatypeProperty ;
                    rdfs:domain :ReconfigurationAction ;
                    rdfs:range rdfs:Literal ;
                    rdfs:comment "Represents the relation between a ReconfiguationAction and the literal (value) it changes a ConfigurableParameter to."@en ;
                    rdfs:label "configuresNewValue"@en .


###  http://www.semanticweb.org/ivans/ontologies/2025/ruleless-digital-twins/hasIdentifier
:hasIdentifier rdf:type owl:DatatypeProperty ;
               rdfs:range xsd:string ;
               rdfs:comment "Represents a relation from a thing to its identifier."@en ;
               rdfs:label "hasIdentifier"@en .


###  http://www.semanticweb.org/ivans/ontologies/2025/ruleless-digital-twins/hasSimulationFidelitySeconds
:hasSimulationFidelitySeconds rdf:type owl:DatatypeProperty ;
                              rdfs:domain :FmuModel ;
                              rdfs:range xsd:int ;
                              rdfs:comment "Represents the fidelity of the simulation models (FMUs) with respect to the equations they contain."@en ;
                              rdfs:label "hasSimulationFidelitySeconds"@en .


###  http://www.semanticweb.org/ivans/ontologies/2025/ruleless-digital-twins/hasTimeLimit
:hasTimeLimit rdf:type owl:DatatypeProperty ;
              rdfs:range xsd:duration ;
              rdfs:comment "Represents a time limit on the duration of the Strategy."@en ;
              rdfs:label "hasTimeLimit"@en .


###  http://www.semanticweb.org/ivans/ontologies/2025/ruleless-digital-twins/hasURI
:hasURI rdf:type owl:DatatypeProperty ;
        rdfs:domain :FmuModel ;
        rdfs:range xsd:anyURI ;
        rdfs:comment "Refers to an FMUs URI."@en ;
        rdfs:label "hasURI"@en .


###  http://www.semanticweb.org/ivans/ontologies/2025/ruleless-digital-twins/hasValue
:hasValue rdf:type owl:DatatypeProperty ;
          rdfs:range rdfs:Literal ;
          rdfs:comment "Describes a relation to a specific value (of a specific type) contained by a property or an Input/Output parameter."@en ;
          rdfs:label "hasValue"@en .


###  http://www.semanticweb.org/ivans/ontologies/2025/ruleless-digital-twins/hasValueConstraint
:hasValueConstraint rdf:type owl:DatatypeProperty ;
                    rdfs:range rdfs:Literal ;
                    rdfs:comment "Represents the relation between a thing and its defined range of values."@en ;
                    rdfs:label "hasValueConstraint"@en .


###  http://www.semanticweb.org/ivans/ontologies/2025/ruleless-digital-twins/reachedInMaximumSeconds
:reachedInMaximumSeconds rdf:type owl:DatatypeProperty ;
                         rdfs:domain :OptimalCondition ;
                         rdfs:range xsd:int ;
                         rdfs:comment "Represents the maximum amount of time in seconds to reach an OptimalCondition."@en ;
                         rdfs:label "reachedInMaximumSeconds"@en .


###  http://www.semanticweb.org/ivans/ontologies/2025/ruleless-digital-twins/setsActuatorToState
:setsActuatorToState rdf:type owl:DatatypeProperty ;
                     rdfs:domain :ActuationAction ;
                     rdfs:range rdfs:Literal .


#################################################################
#    Classes
#################################################################

###  http://www.semanticweb.org/ivans/ontologies/2025/ruleless-digital-twins/Action
:Action rdf:type owl:Class ;
        rdfs:comment "Represents a single system Action."@en ;
        rdfs:label "Action"@en .


###  http://www.semanticweb.org/ivans/ontologies/2025/ruleless-digital-twins/ActionValueGenerator
:ActionValueGenerator rdf:type owl:Class ;
                      rdfs:subClassOf <http://www.w3.org/ns/sosa/Procedure> ,
                                      [ rdf:type owl:Restriction ;
                                        owl:onProperty <http://www.w3.org/ns/ssn/hasInput> ;
                                        owl:qualifiedCardinality "1"^^xsd:nonNegativeInteger ;
                                        owl:onClass :Effect
                                      ] ,
                                      [ rdf:type owl:Restriction ;
                                        owl:onProperty <http://www.w3.org/ns/ssn/hasOutput> ;
                                        owl:cardinality "1"^^xsd:nonNegativeInteger
                                      ] ;
                      rdfs:comment "Represents a specific Procedure that generates concrete Action values. For example, the number of ActuatorStates might be unknown for a certain Actuator, so a Procedure should specify them for concrete ActuationActions. Likewise, ConfigurableParameter values should be specified for concrete ReconfigurationActions."@en ;
                      rdfs:label "ActionValueGenerator"@en .


###  http://www.semanticweb.org/ivans/ontologies/2025/ruleless-digital-twins/ActuationAction
:ActuationAction rdf:type owl:Class ;
                 rdfs:subClassOf :Action ,
                                 [ rdf:type owl:Restriction ;
                                   owl:onProperty :hasActuator ;
                                   owl:qualifiedCardinality "1"^^xsd:nonNegativeInteger ;
                                   owl:onClass <http://www.w3.org/ns/sosa/Actuator>
                                 ] ,
                                 [ rdf:type owl:Restriction ;
                                   owl:onProperty :setsActuatorToState ;
                                   owl:cardinality "1"^^xsd:nonNegativeInteger
                                 ] ;
                 owl:disjointWith :ReconfigurationAction ;
                 rdfs:comment "Represents a single system Action with an actuation, either for optimization or regaining optimal conditions."@en ;
                 rdfs:label "ActuationAction"@en .


###  http://www.semanticweb.org/ivans/ontologies/2025/ruleless-digital-twins/ActuationValueGenerator
:ActuationValueGenerator rdf:type owl:Class ;
                         rdfs:subClassOf :ActionValueGenerator ,
                                         [ rdf:type owl:Restriction ;
                                           owl:onProperty <http://www.w3.org/ns/ssn/hasInput> ;
                                           owl:qualifiedCardinality "1"^^xsd:nonNegativeInteger ;
                                           owl:onClass <http://www.w3.org/ns/sosa/Actuator>
                                         ] .


###  http://www.semanticweb.org/ivans/ontologies/2025/ruleless-digital-twins/ConfigurableParameter
:ConfigurableParameter rdf:type owl:Class ;
                       rdfs:subClassOf <http://www.w3.org/ns/ssn/Input> ,
                                       <http://www.w3.org/ns/ssn/Property> ,
                                       [ rdf:type owl:Restriction ;
                                         owl:onProperty :enacts ;
                                         owl:minQualifiedCardinality "1"^^xsd:nonNegativeInteger ;
                                         owl:onClass :PropertyChangeByReconfiguration
                                       ] ;
                       rdfs:comment "A parameter not directly observable or actuatable but rather used for configuring an an Input to a System or Procedure."@en ;
                       rdfs:label "ConfigurableParameter"@en .


###  http://www.semanticweb.org/ivans/ontologies/2025/ruleless-digital-twins/Effect
:Effect rdf:type owl:Class ;
        rdfs:comment "The type of effect on the value of a property."@en ;
        rdfs:label "Effect"@en .


###  http://www.semanticweb.org/ivans/ontologies/2025/ruleless-digital-twins/FmuModel
:FmuModel rdf:type owl:Class ;
          rdfs:subClassOf <http://www.w3.org/ns/sosa/Procedure> ,
                          [ rdf:type owl:Restriction ;
                            owl:onProperty :hasSimulationFidelitySeconds ;
                            owl:qualifiedCardinality "1"^^xsd:nonNegativeInteger ;
                            owl:onDataRange xsd:int
                          ] ,
                          [ rdf:type owl:Restriction ;
                            owl:onProperty :hasURI ;
                            owl:qualifiedCardinality "1"^^xsd:nonNegativeInteger ;
                            owl:onDataRange xsd:anyURI
                          ] ;
          rdfs:comment "Represents a simulation model in the form of a Functional Mock-up Unit (FMU)."@en ;
          rdfs:label "FmuModel"@en .


###  http://www.semanticweb.org/ivans/ontologies/2025/ruleless-digital-twins/OptimalCondition
:OptimalCondition rdf:type owl:Class ;
                  rdfs:subClassOf [ rdf:type owl:Restriction ;
                                    owl:onProperty <http://www.w3.org/ns/ssn/forProperty> ;
                                    owl:qualifiedCardinality "1"^^xsd:nonNegativeInteger ;
                                    owl:onClass <http://www.w3.org/ns/ssn/Property>
                                  ] ,
                                  [ rdf:type owl:Restriction ;
                                    owl:onProperty :hasValueConstraint ;
                                    owl:cardinality "1"^^xsd:nonNegativeInteger
                                  ] ,
                                  [ rdf:type owl:Restriction ;
                                    owl:onProperty :reachedInMaximumSeconds ;
                                    owl:maxQualifiedCardinality "1"^^xsd:nonNegativeInteger ;
                                    owl:onDataRange xsd:int
                                  ] ;
                  rdfs:comment "An optimal property condition, such as a desired value range definition. For example, an optimal temperature condition of a room could be defined as values greater than 18 and lower than 22 degrees Celsius."@en ;
                  rdfs:label "OptimalCondition"@en .


###  http://www.semanticweb.org/ivans/ontologies/2025/ruleless-digital-twins/PropertyChange
:PropertyChange rdf:type owl:Class ;
                rdfs:subClassOf [ rdf:type owl:Restriction ;
                                  owl:onProperty :affectsPropertyWith ;
                                  owl:qualifiedCardinality "1"^^xsd:nonNegativeInteger ;
                                  owl:onClass :Effect
                                ] ,
                                [ rdf:type owl:Restriction ;
                                  owl:onProperty <http://www.w3.org/ns/ssn/forProperty> ;
                                  owl:qualifiedCardinality "1"^^xsd:nonNegativeInteger ;
                                  owl:onClass <http://www.w3.org/ns/ssn/Property>
                                ] ;
                rdfs:comment "Represents a specific property change in a given system, either via a changed configuration property or an actuation on an observable one."@en ;
                rdfs:label "PropertyChange"@en .


###  http://www.semanticweb.org/ivans/ontologies/2025/ruleless-digital-twins/PropertyChangeByActuation
:PropertyChangeByActuation rdf:type owl:Class ;
                           rdfs:subClassOf :PropertyChange ,
                                           [ rdf:type owl:Restriction ;
                                             owl:onProperty :enactedBy ;
                                             owl:minQualifiedCardinality "1"^^xsd:nonNegativeInteger ;
                                             owl:onClass <http://www.w3.org/ns/sosa/Actuator>
                                           ] ;
                           owl:disjointWith :PropertyChangeByReconfiguration ;
                           rdfs:comment "Represents a specific PropertyChange as a result of actuating on the respective Property."@en ;
                           rdfs:label "PropertyChangeByActuation"@en .


###  http://www.semanticweb.org/ivans/ontologies/2025/ruleless-digital-twins/PropertyChangeByReconfiguration
:PropertyChangeByReconfiguration rdf:type owl:Class ;
                                 rdfs:subClassOf :PropertyChange ,
                                                 [ rdf:type owl:Restriction ;
                                                   owl:onProperty :enactedBy ;
                                                   owl:minQualifiedCardinality "1"^^xsd:nonNegativeInteger ;
                                                   owl:onClass :ConfigurableParameter
                                                 ] ,
                                                 [ rdf:type owl:Restriction ;
                                                   owl:onProperty :alteredBy ;
                                                   owl:qualifiedCardinality "1"^^xsd:nonNegativeInteger ;
                                                   owl:onClass :Effect
                                                 ] ;
                                 rdfs:comment "Represents a specific PropertyChange as a result of reconfiguring a related ConfigurableProperty."@en ;
                                 rdfs:label "PropertyChangeByReconfiguration"@en .


###  http://www.semanticweb.org/ivans/ontologies/2025/ruleless-digital-twins/ReconfigurationAction
:ReconfigurationAction rdf:type owl:Class ;
                       rdfs:subClassOf :Action ,
                                       [ rdf:type owl:Restriction ;
                                         owl:onProperty <http://www.w3.org/ns/ssn/forProperty> ;
                                         owl:qualifiedCardinality "1"^^xsd:nonNegativeInteger ;
                                         owl:onClass :ConfigurableParameter
                                       ] ,
                                       [ rdf:type owl:Restriction ;
                                         owl:onProperty :configuresNewValue ;
                                         owl:cardinality "1"^^xsd:nonNegativeInteger
                                       ] ;
                       rdfs:comment "Represents a single system Action with a parameter reconfiguration, either for optimization or regaining optimal conditions."@en ;
                       rdfs:label "ReconfigurationAction"@en .


###  http://www.semanticweb.org/ivans/ontologies/2025/ruleless-digital-twins/ReconfigurationValueGenerator
:ReconfigurationValueGenerator rdf:type owl:Class ;
                               rdfs:subClassOf :ActionValueGenerator ,
                                               [ rdf:type owl:Restriction ;
                                                 owl:onProperty <http://www.w3.org/ns/ssn/hasInput> ;
                                                 owl:qualifiedCardinality "1"^^xsd:nonNegativeInteger ;
                                                 owl:onClass :ConfigurableParameter
                                               ] .


###  http://www.w3.org/ns/sosa/Actuator
<http://www.w3.org/ns/sosa/Actuator> rdfs:subClassOf [ rdf:type owl:Restriction ;
                                                       owl:onProperty :enacts ;
                                                       owl:minQualifiedCardinality "1"^^xsd:nonNegativeInteger ;
                                                       owl:onClass :PropertyChangeByActuation
                                                     ] .


###  http://www.w3.org/ns/sosa/ObservableProperty
<http://www.w3.org/ns/sosa/ObservableProperty> rdfs:subClassOf [ rdf:type owl:Restriction ;
                                                                 owl:onProperty :hasValue ;
                                                                 owl:cardinality "1"^^xsd:nonNegativeInteger
                                                               ] .


###  http://www.w3.org/ns/sosa/Platform
<http://www.w3.org/ns/sosa/Platform> rdfs:subClassOf [ rdf:type owl:Restriction ;
                                                       owl:onProperty :optimizesFor ;
                                                       owl:minQualifiedCardinality "1"^^xsd:nonNegativeInteger ;
                                                       owl:onClass :PropertyChange
                                                     ] ,
                                                     [ rdf:type owl:Restriction ;
                                                       owl:onProperty <http://www.w3.org/ns/ssn/implements> ;
                                                       owl:minQualifiedCardinality "1"^^xsd:nonNegativeInteger ;
                                                       owl:onClass :OptimalCondition
                                                     ] ,
                                                     [ rdf:type owl:Restriction ;
                                                       owl:onProperty :hasSimulationModel ;
                                                       owl:qualifiedCardinality "1"^^xsd:nonNegativeInteger ;
                                                       owl:onClass <http://www.w3.org/ns/sosa/Procedure>
                                                     ] .


#################################################################
#    Individuals
#################################################################

###  http://www.semanticweb.org/ivans/ontologies/2025/ruleless-digital-twins/ValueDecrease
:ValueDecrease rdf:type owl:NamedIndividual ,
                        :Effect .


###  http://www.semanticweb.org/ivans/ontologies/2025/ruleless-digital-twins/ValueIncrease
:ValueIncrease rdf:type owl:NamedIndividual ,
                        :Effect .


###  Generated by the OWL API (version 4.5.29.2024-05-13T12:11:03Z) https://github.com/owlcs/owlapi
